TransVal/sexp.v
@@ -1,11 +1,10 @@
 Require Import List NPeano Decidable.
-Require Import IL bitvec.
+Require Import IL Val bitvec.
 
 Set Implicit Arguments.
 
 (* An smt environment must be defined on every variable that occurs in the formula.
 Hence it is safe to not use options here *)
-Definition senv:Type := var -> bitvec.
 
 (** Define SMT expressions on bitvectors. **)
 Inductive sexp :=
@@ -31,7 +30,12 @@ evalSexp evaluates an SMT expression given an environment that must! be total on
 every variable that may occur in a formula. 
 **)
 
-Fixpoint evalSexp (E: senv)(s:sexp): bitvec :=
+Definition evalSexp E s : bitvec :=
+match exp_eval E s with
+|Some v => v
+|None => default_val
+end.
+(*
 match s with
 |splus a b 
   => bvAdd ( evalSexp E a) (evalSexp E b) 
@@ -53,6 +57,7 @@ match s with
 | svar v
   => E v
 end.
+*)
 
 (* Not needed stuff begins here *)
 (*
