TransVal/smt.v
@@ -4,7 +4,7 @@ Require Import IL Exp Val  sexp bitvec.
 Set Implicit Arguments.
 
 (** Define what an argument list is **)
-Definition arglst := list sexp.
+Definition arglst := list exp.
 
 Definition vallst := list bitvec.
 
@@ -16,11 +16,11 @@ Inductive smt :Type :=
 | smtAnd: smt -> smt -> smt
 | smtOr: smt -> smt -> smt
 | smtNeg: smt -> smt
-| ite: sexp -> smt -> smt -> smt
+| ite: exp -> smt -> smt -> smt
 | smtImp: smt -> smt -> smt
-| constr: sexp -> sexp -> smt
+| constr: exp -> exp -> smt
 | funcApp: pred -> arglst -> smt
-|smtReturn: sexp -> smt
+|smtReturn:  exp -> smt
 |smtFalse: smt.
 
 (** Now define the parameters for the translation function **)
@@ -37,33 +37,30 @@ match o1, o2 with
 end.
 
 (** Function to generate the guard expression for one expression **)
-Fixpoint undef (e:sexp) :=
+Fixpoint undef e :=
 match e with
-|splus a b 
- => combine (undef a) (undef b)
-|ssub a b
- => combine (undef a) (undef b)
-|smult a b
- => combine (undef a) (undef b)
-|sdiv a b
- => let o1 := undef a in
-    let o2 := undef b in
-      match combine o1 o2 with
-          | Some v => Some (smtAnd v (smtNeg (constr b (sconst (O::nil)))))
-          | None => Some (smtNeg (constr b (sconst (O::nil))))
+|BinOp n a b 
+ => match n with 
+        | 5 => match combine (undef a) (undef b) with 
+                 | Some c => Some (smtAnd (smtNeg (constr b (Con (zext k (O::nil))))) c )
+                 | None =>  Some (smtNeg (constr b (Con (zext k (O::nil)))))
+               end
+        | _ => combine (undef a) (undef b)
     end
-| sneg a
- => undef a
-| seq a b
-  => combine (undef a) (undef b)
-|sconst c
+|UnOp n a
+ => match n with
+        | 0 => undef a
+        | 1 => undef a
+        | _ => None
+    end
+|Con v
  => None
-|svar v
+|Var v
  => None
 end. 
 
 (** Now the function that generates the guarding expressions for the smt translation function **)
-Fixpoint guard (p:pol) (e:sexp) (cont:smt) :=
+Fixpoint guard (p:pol) (e:exp) (cont:smt) :=
 match p, undef e with
 |source, Some g
  => smtAnd g cont
@@ -81,8 +78,9 @@ match l with
 | x:: l' => guardList p l' (guard p x cont)
 end.
 
+(*
 (** Define expression translation **)
-Fixpoint translateExp (e:exp) :option sexp :=
+Fixpoint translateExp (e:exp) :option exp :=
 match e with
 |Con v 
  => Some ( sconst v)
@@ -107,7 +105,9 @@ match e with
            |_, _ => None
        end
 end.
+*)
 
+(*
 Fixpoint translateArgs (e:args) : option arglst :=
 match e with
 | nil => Some nil
@@ -117,57 +117,56 @@ match e with
          |  _, _ => None
      end
 end.
-
+*)
 
 Fixpoint translateStmt (s:stmt) (p:pol) :smt :=
 match s, p with
 (*let x = e in s' *)
 | stmtExp x e s', _ 
-  => let e' := translateExp e in
-        let x' := translateExp (Var x) in (* TODO: is this ok ? Hack from var to exp*)
+  => (*let e' := translateExp e in
+        let x' := translateExp (Var x) in (* TODO: is this ok ? Hack from var to exp*) *)
         let smt' := translateStmt s' p in
-        match x', e' with
-          | Some x' , Some v => guard  p  v   (smtAnd ( constr x' v) smt')
-          | _, _ => smtFalse
-        end
+        guard  p  e   (smtAnd ( constr (Var x) e) smt')
+(*          | _, _ => smtFalse *)
+(*        end *)
 (* if e then s else t *)
 | stmtIf e s t, _
   => let s' := translateStmt s p in
         let t' := translateStmt t p in
-        let e' := translateExp e in
-        match e' with
-            | Some v => guard  p  v ( ite v s' t')
-            | _ => smtFalse
-        end
+       (* let e' := translateExp e in *)
+       (* match e' with 
+            | Some v =>*) guard  p  e ( ite e s' t')
+(*            | _ => smtFalse *)
+(*        end *)
 (* fun f x = t in s *)
 |  stmtLet x  t s, _ => smtFalse (* TODO *)
 (* extern ?? *)
 |  stmtExtern x f Y s, _ => smtFalse (* TODO *)
 (* f e, s*)
 | stmtGoto f e, source 
-  => match translateArgs e with
-         |Some l =>  guardList source l (funcApp f l)
-         | None => smtFalse
-     end
+  => (* match translateArgs e with 
+         |Some l =>  *) guardList source e (funcApp f e)
+(*         | None => smtFalse 
+     end *)
 (* f e, t *)
 | stmtGoto f e, target  
-  => match translateArgs e with
-         | Some l => guardList target  l  ( smtNeg (funcApp f l ))
-         | None => smtFalse
-     end
+  => (* match translateArgs e with
+         | Some l => *) guardList target  e  ( smtNeg (funcApp f e ))
+(*         | None => smtFalse
+     end *)
 | stmtReturn e, source 
-  => match translateExp e with
-       |Some v => guard source  v  (smtReturn v)
-       | None => smtFalse
-     end
+  => (* match translateExp e with
+       |Some v =>*) guard source  e  (smtReturn e)
+(*       | None => smtFalse 
+     end *)
 | stmtReturn e, target 
-  => match translateExp e with
-         | Some v => guard  target  v ( smtNeg (smtReturn v))
-         | None => smtFalse
-     end
+  => (*match translateExp e with
+         | Some v =>*) guard  target  e ( smtNeg (smtReturn e))
+(*         | None => smtFalse
+     end*)
 end.
 
-Fixpoint evalList (E:senv) (e:arglst) : vallst :=
+Fixpoint evalList E (e:arglst) : vallst :=
 match e with
 |nil =>  nil
 |x::e' => (evalSexp E x) :: ( evalList E e')
@@ -178,7 +177,7 @@ F f e.
 
 (** models relation for smt. No need for options here too, because if models can be evaluated by an environment,
 every variable must have been defined. **)
-Fixpoint models (F:pred ->vallst->bool)(E:senv) (s:smt) : Prop:=
+Fixpoint models (F:pred ->vallst->bool) E (s:smt) : Prop:=
 match s with
   |smtAnd a b 
    => (models F E a) /\ (models F E b)
