TransVal/terminates.v
@@ -3,9 +3,9 @@ Require Import IL smt.
 Set Implicit Arguments.
 
 Inductive terminates :F.state -> F.state -> Prop :=
-|terminatesReturn L E e b v:
-   translateExp e = ⎣b⎦ 
-   -> exp_eval E e = ⎣v⎦
+|terminatesReturn L E e v:
+(*   translateExp e = ⎣b⎦  *)
+   exp_eval E e = ⎣v⎦
    -> terminates (L, E, stmtReturn e)   (L  , E , stmtReturn e)
 |terminatesStep sigma sigma' sigma'' a:
    F.step sigma a sigma'
