TransVal/transval.v
@@ -1,137 +1,211 @@
 Require Import List.
 Require Import IL Annotation AutoIndTac Bisim Exp MoreExp Coherence Fresh sexp smt nofun terminates bitvec.
 
-Definition lift_env (E:onv val)  :=
-fun x => match E x with 
-|Some v => v
-| _ => default_val
-end.
-
-(*
-Lemma evals_impl_subexp_eval:
-forall E e o e1 e2 v ,
-e = BinOp o e1 e2
--> exp_eval E e = Some v
--> exists v1 v2, exp_eval E e1 = Some v1/\ exp_eval E e2 = Some v2.
+Lemma bvEq_equiv_eq:
+forall b1 b2, toBool(bvEq b1 b2) <-> eq b1 b2.
 
 Proof.
-intros. rewrite H in H0. simpl in H0.  case_eq (exp_eval E e1); case_eq (exp_eval E e2); intros.
-- exists v1; exists v0; eauto.
--  rewrite H2 in H0. rewrite H1 in H0. simpl in H0. exfalso; discriminate H0.
--  *)
-
- Lemma guard_true_if_eval:
-forall F E e x s v,  
- translateExp e = Some x 
--> undef x = Some s 
-->  exp_eval E e = Some v 
-->  models F (lift_env E) s.
-
-Proof.
-intros. general induction e; simpl in *.
--  destruct u.
-  + destruct( translateExp e).
-    * inversion H. rewrite <- H3 in H0. monad_inv H1. simpl in H0.  eapply IHe; eauto.
-    * exfalso; discriminate H.
-  + exfalso. discriminate H.
--  monad_inv H1. destruct  (translateExp e1); destruct (translateExp e2).
-   + destruct b. 
-     * inversion H. rewrite <- H2 in H0.  simpl in H0.  case_eq (undef s0); case_eq (undef s1); intros; simpl.
-       { unfold combine in H0.   rewrite H1 in H0; rewrite H3 in H0. inversion H0; simpl; split.
-         - eapply IHe1; eauto.
-         - eapply IHe2; eauto.
-       }
-       { unfold combine in H0; rewrite H1 in H0; rewrite H3 in H0; inversion H0. eapply IHe1; eauto. rewrite <- H5; eauto. }
-       { unfold combine in H0; rewrite H1 in H0; rewrite H3 in H0; inversion H0. eapply IHe2; eauto. rewrite <- H5; eauto. }
-       { unfold combine in H0; rewrite H1 in H0; rewrite H3 in H0; inversion H0. }
-     *  destruct b.
-        { inversion H; rewrite <- H2 in H0. simpl in H0; case_eq(undef s0); case_eq (undef s1); intros; simpl.
-          - unfold combine in H0. rewrite H1 in H0; rewrite H3 in H0. inversion H0; simpl; split.
-            + eapply IHe1; eauto.
-            + eapply IHe2; eauto.
-          - unfold combine in H0; rewrite H1 in H0; rewrite H3 in H0; inversion H0. eapply IHe1; eauto. rewrite <- H5; eauto. 
-          - unfold combine in H0; rewrite H1 in H0; rewrite H3 in H0; inversion H0. eapply IHe2; eauto. rewrite <- H5; eauto. 
-          - unfold combine in H0; rewrite H1 in H0; rewrite H3 in H0; inversion H0. 
-        }
-        { destruct b. 
-          -  inversion H; rewrite <- H2 in H0. simpl in H0; case_eq(undef s0); case_eq (undef s1); intros; simpl.
-             + unfold combine in H0. rewrite H1 in H0; rewrite H3 in H0. inversion H0; simpl; split.
-               * eapply IHe1; eauto.
-               * eapply IHe2; eauto.
-             + unfold combine in H0; rewrite H1 in H0; rewrite H3 in H0; inversion H0. eapply IHe1; eauto. rewrite <- H5; eauto. 
-             + unfold combine in H0; rewrite H1 in H0; rewrite H3 in H0; inversion H0. eapply IHe2; eauto. rewrite <- H5; eauto. 
-             + unfold combine in H0; rewrite H1 in H0; rewrite H3 in H0; inversion H0. 
-          - destruct b.
-            + inversion H; rewrite <- H2 in H0. simpl in H0; case_eq(undef s0); case_eq (undef s1); intros; simpl.
-              * unfold combine in H0. rewrite H1 in H0; rewrite H3 in H0. inversion H0; simpl; split.
-              {  eapply IHe1; eauto. }
-              { eapply IHe2; eauto. }
-              * unfold combine in H0; rewrite H1 in H0; rewrite H3 in H0; inversion H0. eapply IHe1; eauto. rewrite <- H5; eauto. 
-              * unfold combine in H0; rewrite H1 in H0; rewrite H3 in H0; inversion H0. eapply IHe2; eauto. rewrite <- H5; eauto. 
-              * unfold combine in H0; rewrite H1 in H0; rewrite H3 in H0; inversion H0. 
-            + destruct b.
-              * inversion H; rewrite <- H2 in H0. simpl in H0; case_eq(undef s0); case_eq (undef s1); intros; simpl.
-                { unfold combine in H0. rewrite H1 in H0; rewrite H3 in H0. inversion H0; simpl; split. 
-                  - eapply IHe1; eauto.
-                  - eapply IHe2; eauto. }
-                { unfold combine in H0; rewrite H1 in H0; rewrite H3 in H0; inversion H0. eapply IHe1; eauto. rewrite <- H5; eauto. }
-                { unfold combine in H0; rewrite H1 in H0; rewrite H3 in H0; inversion H0. eapply IHe2; eauto. rewrite <- H5; eauto. }
-                { unfold combine in H0; rewrite H1 in H0; rewrite H3 in H0; inversion H0. }
-              * exfalso; discriminate H.
-          }
-   + exfalso; discriminate H.
-   + exfalso; discriminate H.
-   + exfalso; discriminate H.
+intros; split; intros.
+- general induction b1; destruct b2.
+  + reflexivity.
+  + simpl in H. exfalso; assumption.
+  + simpl in H. exfalso; assumption.
+  + destruct a,b.
+    * simpl. simpl in H. f_equal. eapply IHb1. assumption.
+    * simpl in H; exfalso; assumption.
+    * simpl in H; exfalso; assumption.
+    * f_equal. simpl in H; eapply IHb1; assumption.
+- general induction b1.
+  + simpl. econstructor.
+  + destruct a.
+    * simpl. eapply (IHb1 b1). reflexivity.
+    * simpl. eapply (IHb1 b1); reflexivity.
 Qed.
 
-Lemma toBool_if_val2bool:
-forall E e v c x,  exp_eval E e = Some v -> val2bool v = c -> translateExp e = Some x -> toBool(evalSexp (lift_env E) x) = c.
+Lemma not_zero:
+ forall b, bvZero b = false ->  b  <> zext k (O::nil).
+
+Proof.
+ intros. general induction b.
+ destruct a; simpl; hnf; intros. 
+ - rewrite H0 in H. simpl in H. discriminate H.
+- rewrite H0 in H.  simpl in H; discriminate H.
+Qed.
+ 
+Lemma zext_nil_eq_sext:
+  forall k, sext k nil O = zext k nil.
+
+Proof.
+  intros; general induction k.
+  - simpl. reflexivity.
+  - simpl. f_equal; eauto; assumption.
+Qed.
+
+Lemma bvEq_eq_refl:
+forall a, val2bool (bvEq a a) = true.
+
+Proof.
+intros; general induction a.
+- eauto.
+- simpl. rewrite IHa in *. destruct a; simpl; rewrite IHa; reflexivity.
+Qed.
+
+Lemma not_zero_implies_uneq:
+forall a b, bvZero a = false ->b = zext k (O::nil) ->  val2bool(bvEq a b) = false.
 
 Proof. 
-intros. induction e; simpl in *.
-- inversion H1. simpl. inversion H.  
+intros.  induction a.
+- simpl.  rewrite H0. reflexivity.
+- destruct a. 
+  + simpl in H. specialize (IHa H).  admit.
+  + simpl in H. rewrite H0. simpl. reflexivity.
+Qed.
+
+ Lemma guard_true_if_eval:
+forall F E e s v,  
+ (*translateExp e = Some x  *)
+ exp_eval E e = Some v 
+->  undef e = Some s 
+->  models F E s.
+
+Proof.
+intros. general induction e; simpl.
+- simpl in *. monad_inv H. destruct u.
+  + apply (IHe F E s x); eauto.
+  + destruct u.
+    *  apply (IHe F E s x); eauto. 
+    * exfalso; discriminate H0.
+- simpl in H.  monad_inv H.  simpl in H0. destruct b.
+  +  case_eq (undef e1); case_eq (undef e2); intros.
+     *  rewrite H in H0; rewrite H1 in H0. simpl in H0. inversion H0. simpl; split.
+        { eapply IHe1; eauto. }
+        { eapply IHe2; eauto. }
+     * rewrite H in H0; rewrite H1 in H0; simpl in H0; inversion H0; simpl. eapply IHe1; eauto. rewrite <- H0; eauto.
+     *rewrite H in H0; rewrite H1 in H0; simpl in H0; inversion H0; simpl. eapply IHe2; eauto. rewrite <- H0; eauto.
+     * rewrite H in H0; rewrite H1 in H0; simpl in H0;  simpl. exfalso; discriminate H0.
+  + destruct b.
+    *  case_eq (undef e1); case_eq (undef e2); intros.
+     {  rewrite H in H0; rewrite H1 in H0. simpl in H0. inversion H0. simpl; split.
+        - eapply IHe1; eauto. 
+        - eapply IHe2; eauto. }
+     { rewrite H in H0; rewrite H1 in H0; simpl in H0; inversion H0; simpl. eapply IHe1; eauto. rewrite <- H0; eauto. }
+     { rewrite H in H0; rewrite H1 in H0; simpl in H0; inversion H0; simpl. eapply IHe2; eauto. rewrite <- H0; eauto. }
+     { rewrite H in H0; rewrite H1 in H0; simpl in H0;  simpl. exfalso; discriminate H0. }
+    * destruct b. 
+      { case_eq (undef e1); case_eq (undef e2); intros.
+        -  rewrite H in H0; rewrite H1 in H0. simpl in H0. inversion H0. simpl; split.
+           + eapply IHe1; eauto. 
+           + eapply IHe2; eauto. 
+        - rewrite H in H0; rewrite H1 in H0; simpl in H0; inversion H0; simpl. eapply IHe1; eauto. rewrite <- H0; eauto.
+        - rewrite H in H0; rewrite H1 in H0; simpl in H0; inversion H0; simpl. eapply IHe2; eauto. rewrite <- H0; eauto.
+        - rewrite H in H0; rewrite H1 in H0; simpl in H0;  simpl. exfalso; discriminate H0. }
+      { destruct b. 
+        -  case_eq (undef e1); case_eq (undef e2); intros.
+           +  rewrite H in H0; rewrite H1 in H0. simpl in H0. inversion H0. simpl; split.
+              * eapply IHe1; eauto. 
+              * eapply IHe2; eauto. 
+           + rewrite H in H0; rewrite H1 in H0; simpl in H0; inversion H0; simpl. eapply IHe1; eauto. rewrite <- H0; eauto.
+           + rewrite H in H0; rewrite H1 in H0; simpl in H0; inversion H0; simpl. eapply IHe2; eauto. rewrite <- H0; eauto.
+            +rewrite H in H0; rewrite H1 in H0; simpl in H0;  simpl. exfalso; discriminate H0.
+        - destruct b.
+          +  case_eq (undef e1); case_eq (undef e2); intros.
+             *  rewrite H in H0; rewrite H1 in H0. simpl in H0. inversion H0. simpl; split.
+                { eapply IHe1; eauto. }
+                { eapply IHe2; eauto. }
+             * rewrite H in H0; rewrite H1 in H0; simpl in H0; inversion H0; simpl. eapply IHe1; eauto. rewrite <- H0; eauto.
+             *rewrite H in H0; rewrite H1 in H0; simpl in H0; inversion H0; simpl. eapply IHe2; eauto. rewrite <- H0; eauto.
+             * rewrite H in H0; rewrite H1 in H0; simpl in H0;  simpl. exfalso; discriminate H0.
+          + destruct b.
+            * case_eq (undef e1); case_eq (undef e2); intros.
+              {  rewrite H in H0; rewrite H1 in H0. simpl in H0. inversion H0.   unfold binop_eval in EQ2.  clear H0. unfold bvDiv in EQ2. simpl. split.
+                 - case_eq(bvZero x0).
+                   + intros.  rewrite H0 in EQ2.  exfalso; discriminate EQ2. 
+                   + intros A.   unfold evalSexp. intros. clear H3. clear EQ2.  hnf in H0.  rewrite EQ1 in H0.  simpl in H0. simpl  in A.  
+                     erewrite  not_zero_implies_uneq in H0; eauto.   
+                 - split.
+                   + eapply IHe1; eauto.
+                   + eapply IHe2; eauto.  }
+                 { rewrite H in H0; rewrite H1 in H0; simpl in H0. inversion H0. unfold binop_eval in EQ2. clear H0. unfold bvDiv in EQ2. simpl. split.
+                 - case_eq(bvZero x0).
+                   + intros.  rewrite H0 in EQ2.  exfalso; discriminate EQ2. 
+                   + intros A.   unfold evalSexp. intros. clear H3. clear EQ2.  hnf in H0. rewrite EQ1 in H0.  simpl in H0. simpl  in A.  
+                     erewrite  not_zero_implies_uneq in H0; eauto.   
+                 -  eapply IHe1; eauto. }
+                 { rewrite H in H0; rewrite H1 in H0; simpl in H0. inversion H0. unfold binop_eval in EQ2. clear H0. unfold bvDiv in EQ2. simpl. split.
+                 - case_eq(bvZero x0).
+                   + intros.  rewrite H0 in EQ2.  exfalso; discriminate EQ2. 
+                   + intros A.   unfold evalSexp. intros. clear H3. clear EQ2.  hnf in H0.  rewrite EQ1 in H0.  simpl in H0. simpl  in A.  
+                     erewrite  not_zero_implies_uneq in H0; eauto.   
+                 -  eapply IHe2; eauto. }
+                 { rewrite H in H0; rewrite H1 in H0; simpl in H0. inversion H0. unfold binop_eval in EQ2. clear H0. unfold bvDiv in EQ2. simpl.
+                   case_eq(bvZero x0).
+                   - intros.  rewrite H0 in EQ2.  exfalso; discriminate EQ2. 
+                   - intros A.   unfold evalSexp. intros. clear H3. clear EQ2.  hnf in H0. rewrite EQ1 in H0.  simpl in H0. simpl  in A.  
+                     erewrite  not_zero_implies_uneq in H0; eauto.    }
+                 * case_eq (undef e1); case_eq (undef e2); intros; simpl.
+                   { rewrite H in H0; rewrite H1 in H0; simpl in H0. inversion H0. simpl; split.
+                     - eapply IHe1; eauto.
+                     - eapply IHe2; eauto. }
+                   { rewrite H in H0; rewrite H1 in H0; simpl in H0. inversion H0. simpl.
+                     - eapply IHe1; eauto. rewrite <- H3. assumption. }
+                   { rewrite H in H0; rewrite H1 in H0; simpl in H0. inversion H0. simpl.
+                     - eapply IHe2; eauto. rewrite <- H3. assumption. }
+                   {  rewrite H in H0; rewrite H1 in H0; simpl in H0. inversion H0. }
+      }
+Qed.
 
 Lemma models_if_eval :
 forall s D E s' E', 
 ssa  s D
--> (forall x, x ∈ fst (getAnn D) -> E x <> None)
--> (forall e, exists v, translateExp e = ⎣v⎦)
+(*-> (forall x, x ∈ fst (getAnn D) -> E x <> None) *)
+(*-> (forall e, exists v, translateExp e = ⎣v⎦) *)
 -> agree_on eq (fst (getAnn D)) E E'
 -> noFun s 
 -> terminates (nil,E, s) (nil, E', s')
-->  models (fun (f:pred) (x:vallst) => true)  (lift_env E')  (translateStmt s source).
+->  models (fun (f:pred) (x:vallst) => true)  E'  (translateStmt s source).
 
 Proof.
 intros.
-general induction H4; simpl.
--  destruct (H3 e). rewrite H6. case_eq (undef x).
+general induction H2; simpl.
+-   case_eq (undef e).
    + simpl; split.
      * eapply (guard_true_if_eval); eauto.
      * econstructor.
    + intros. simpl. econstructor.
 - inversion H. 
-  + simpl. destruct (H2 e). rewrite H11. case_eq (undef x0); intros; simpl; split.
-    *  eapply(guard_true_if_eval (fun (_:pred) (_:vallst) => true) E' e x0 s0 v); eauto.  assert (freeVars e ⊆ (fst (getAnn D))).
-      {  rewrite <- H9 in H0. inversion H0. simpl.  assumption. }
-      { eapply (exp_eval_agree (E:= E)); eauto.  cset_tac. hnf in H3. hnf in H13. hnf. intros. specialize (H3 x1). specialize (H13 x1). exact (H3 (H13 H6)). }
+  + simpl. case_eq (undef e); intros; simpl; split.
+    *  eapply(guard_true_if_eval (fun (_:pred) (_:vallst) => true) E' e s0 v); eauto.  assert (freeVars e ⊆ (fst (getAnn D))).
+      {  rewrite <- H7 in H0. inversion H0. simpl.  assumption. }
+      { eapply (exp_eval_agree (E:= E)); eauto.  cset_tac. hnf in H1. hnf in H10. hnf. intros. specialize (H1 x0). specialize (H10 x0). exact (H1 (H10 H4)). }
     * split; simpl.
-     { unfold lift_env at 1. inversion H4. inversion H7. assert (E' x = Some v).
-       -  admit.
-       - rewrite H20.  assert (evalSexp (lift_env E') x0 = v) by admit.
-        rewrite H21.  erewrite (bvEq_true_eq). econstructor.
-       - (* same as * before *) admit.
-       }
-  { rewrite <- H9 in H0. inversion H0. rewrite <- H9 in H5.  inversion H5.  eapply IHterminates; eauto.
-    - admit.
-    - admit. }
-    * (* same as * before *) admit.
-    * (* same as { before *) admit.
-  + simpl. destruct (H2 e). rewrite H11. case_eq (undef x); intros; simpl; try split.
-    * eapply(guard_true_if_eval (fun (_:pred) (_:vallst) => true) E' e x s0 v); eauto.  assert (freeVars e ⊆ (fst (getAnn D))).
-      {  rewrite <- H9 in H0. inversion H0. simpl.  assumption. }
-      { eapply (exp_eval_agree (E:= E)); eauto.  cset_tac. hnf in H3. hnf in H13. hnf. intros. specialize (H3 x0). specialize (H13 x0). exact (H3 (H13 H6)). }
-    *  
-
+      {  unfold evalSexp.  
+         assert (freeVars e ⊆ fst (getAnn D)) by  (rewrite <- H7 in H0; inversion H0; simpl; assumption).  
+         eapply (exp_eval_agree (E:=E) (E' := E')) in def.
+         - rewrite def.  simpl. (* Wert aus E' für x konstruieren *) admit.
+         - cset_tac. hnf; hnf in H1; hnf in H10. hnf; intros; specialize(H1 x0); specialize (H10 x0); exact (H1 (H10 H4)).  }
+      { rewrite <- H7 in H0.  inversion H0.  eapply (IHterminates b an); eauto.
+        - admit.
+        - rewrite <-  H7 in H3. inversion H3.  assumption. }
+    * unfold evalSexp.
+      assert (freeVars e ⊆ fst (getAnn D)) by  (rewrite <- H7 in H0; inversion H0; simpl; assumption).  
+      eapply (exp_eval_agree (E:=E) (E' := E')) in def.
+      { rewrite def.  simpl. (* Wert aus E' für x konstruieren *) admit. }
+      { cset_tac. hnf; hnf in H1; hnf in H10. hnf; intros; specialize(H1 x0); specialize (H10 x0); exact (H1 (H10 H4)). }
+    *  rewrite <- H7 in H0.  inversion H0.  eapply (IHterminates b an); eauto.
+       { admit. }
+       { rewrite <-  H7 in H3. inversion H3.  assumption. }
+  + simpl.
+    assert (X: models (fun (_: pred) (_ : vallst) => true) E' (ite e (translateStmt b1 source) (translateStmt b2 source))). 
+    * simpl.
+      assert (freeVars e ⊆ fst (getAnn D)) by  (rewrite <- H7 in H0; inversion H0; simpl; assumption).
+      assert (agree_on eq (freeVars e) E E').
+      { cset_tac. hnf. hnf in H1; hnf in H9; hnf; intros; specialize(H1 x); specialize (H9 x); exact (H1 (H9 H4)). }
+      { eapply (exp_eval_agree (E:=E) (E' := E') ) in def; eauto. unfold evalSexp. rewrite def. rewrite condTrue. admit. }
+    * admit.
+  + admit. 
+  + simpl. admit.
+  + rewrite <-  H7 in H3. exfalso. inversion H3.
+  + rewrite <- H7 in H3. exfalso. inversion H3.
 Qed.
 
 Definition smtCheck (s:stmt) (t:stmt) :=
